Vibe proving

rupicola/io/QTyp.fst
@@ -111,61 +111,163 @@ let lem_closed_is_no_fv (e:exp) : Lemma
   [SMTPat (is_closed e)] =
   ()
 
+(** Helper: incrementing the binder depth shifts free variable indices by -1.
+    I.e., fv in free_vars_indx at depth n+1 iff fv+1 in free_vars_indx at depth n. **)
+let rec lem_free_vars_indx_shift (e:exp) (n:nat) :
+  Lemma (ensures forall (fv:var). fv `memP` free_vars_indx e (n+1) <==> (fv+1) `memP` free_vars_indx e n)
+        (decreases e) =
+  match e with
+  | EUnit | ETrue | EFalse | EFileDescr _ | EString _ -> ()
+  | EVar _ -> ()
+  | ELam e' -> lem_free_vars_indx_shift e' (n+1)
+  | EFst e' | ESnd e' | EInl e' | EInr e'
+  | ERead e' | EOpen e' | EClose e' -> lem_free_vars_indx_shift e' n
+  | EApp e1 e2 | EPair e1 e2 | EWrite e1 e2 ->
+    lem_free_vars_indx_shift e1 n;
+    lem_free_vars_indx_shift e2 n;
+    append_memP_forall (free_vars_indx e1 (n+1)) (free_vars_indx e2 (n+1));
+    append_memP_forall (free_vars_indx e1 n) (free_vars_indx e2 n)
+  | EIf e1 e2 e3 ->
+    lem_free_vars_indx_shift e1 n;
+    lem_free_vars_indx_shift e2 n;
+    lem_free_vars_indx_shift e3 n;
+    append_memP_forall (free_vars_indx e1 (n+1) @ free_vars_indx e2 (n+1)) (free_vars_indx e3 (n+1));
+    append_memP_forall (free_vars_indx e1 (n+1)) (free_vars_indx e2 (n+1));
+    append_memP_forall (free_vars_indx e1 n @ free_vars_indx e2 n) (free_vars_indx e3 n);
+    append_memP_forall (free_vars_indx e1 n) (free_vars_indx e2 n)
+  | ECase e1 e2 e3 ->
+    lem_free_vars_indx_shift e1 n;
+    lem_free_vars_indx_shift e2 (n+1);
+    lem_free_vars_indx_shift e3 (n+1);
+    append_memP_forall (free_vars_indx e1 (n+1) @ free_vars_indx e2 (n+2)) (free_vars_indx e3 (n+2));
+    append_memP_forall (free_vars_indx e1 (n+1)) (free_vars_indx e2 (n+2));
+    append_memP_forall (free_vars_indx e1 n @ free_vars_indx e2 (n+1)) (free_vars_indx e3 (n+1));
+    append_memP_forall (free_vars_indx e1 n) (free_vars_indx e2 (n+1))
+
+(** Helper: a "shift-at-depth-n" substitution (identity below n, +1 at/above n)
+    shifts all free variable indices by +1. *)
+#push-options "--split_queries always --z3rlimit 15"
+let rec lem_free_vars_subst_inc (s:sub true) (e:exp) (n:nat) :
+  Lemma
+    (requires
+      (forall (y:var). y < n ==> s y == EVar y) /\
+      (forall (y:var). y >= n ==> s y == EVar (y + 1)))
+    (ensures forall (fv:var). (fv+1) `memP` free_vars_indx (subst s e) n <==> fv `memP` free_vars_indx e n)
+    (decreases e) =
+  match e with
+  | EUnit | ETrue | EFalse | EFileDescr _ | EString _ -> ()
+  | EVar _ -> ()
+  | ELam e' ->
+    let s' = sub_elam s in
+    introduce forall (y:var). y < n+1 ==> s' y == EVar y with begin
+      introduce _ ==> _ with _. begin
+        if y = 0 then () else ()
+      end
+    end;
+    introduce forall (y:var). y >= n+1 ==> s' y == EVar (y + 1) with begin
+      introduce _ ==> _ with _. ()
+    end;
+    lem_free_vars_subst_inc s' e' (n+1)
+  | EFst e' | ESnd e' | EInl e' | EInr e'
+  | ERead e' | EOpen e' | EClose e' ->
+    lem_free_vars_subst_inc s e' n
+  | EApp e1 e2 | EPair e1 e2 | EWrite e1 e2 ->
+    lem_free_vars_subst_inc s e1 n;
+    lem_free_vars_subst_inc s e2 n;
+    append_memP_forall (free_vars_indx (subst s e1) n) (free_vars_indx (subst s e2) n);
+    append_memP_forall (free_vars_indx e1 n) (free_vars_indx e2 n)
+  | EIf e1 e2 e3 ->
+    lem_free_vars_subst_inc s e1 n;
+    lem_free_vars_subst_inc s e2 n;
+    lem_free_vars_subst_inc s e3 n;
+    append_memP_forall (free_vars_indx (subst s e1) n @ free_vars_indx (subst s e2) n) (free_vars_indx (subst s e3) n);
+    append_memP_forall (free_vars_indx (subst s e1) n) (free_vars_indx (subst s e2) n);
+    append_memP_forall (free_vars_indx e1 n @ free_vars_indx e2 n) (free_vars_indx e3 n);
+    append_memP_forall (free_vars_indx e1 n) (free_vars_indx e2 n)
+  | ECase e1 e2 e3 ->
+    lem_free_vars_subst_inc s e1 n;
+    let s' = sub_elam s in
+    introduce forall (y:var). y < n+1 ==> s' y == EVar y with begin
+      introduce _ ==> _ with _. begin
+        if y = 0 then () else ()
+      end
+    end;
+    introduce forall (y:var). y >= n+1 ==> s' y == EVar (y + 1) with begin
+      introduce _ ==> _ with _. ()
+    end;
+    lem_free_vars_subst_inc s' e2 (n+1);
+    lem_free_vars_subst_inc s' e3 (n+1);
+    append_memP_forall (free_vars_indx (subst s e1) n @ free_vars_indx (subst s' e2) (n+1)) (free_vars_indx (subst s' e3) (n+1));
+    append_memP_forall (free_vars_indx (subst s e1) n) (free_vars_indx (subst s' e2) (n+1));
+    append_memP_forall (free_vars_indx e1 n @ free_vars_indx e2 (n+1)) (free_vars_indx e3 (n+1));
+    append_memP_forall (free_vars_indx e1 n) (free_vars_indx e2 (n+1))
+#pop-options
+
 let lem_fv_in_env_varS (g:typ_env) (t:qType) (e:exp) :
   Lemma (fv_in_env g e <==> fv_in_env (extend t g) (subst sub_inc e))
-  = admit ()
+  = lem_free_vars_subst_inc sub_inc e 0
 
 let lem_fv_in_env_lam (g:typ_env) (t:qType) (body:exp) :
   Lemma (fv_in_env (extend t g) body <==>  fv_in_env g (ELam body))
-   = admit ()
+   = lem_free_vars_indx_shift body 0
 
 let lem_fv_in_env_app (g:typ_env) (e1 e2:exp) :
   Lemma ((fv_in_env g e1 /\ fv_in_env g e2) <==> fv_in_env g (EApp e1 e2))
-  = admit ()
+  = append_memP_forall (free_vars e1) (free_vars e2)
 
 let lem_fv_in_env_if (g:typ_env) (e1 e2 e3:exp) :
   Lemma ((fv_in_env g e1 /\ fv_in_env g e2 /\ fv_in_env g e3) <==> fv_in_env g (EIf e1 e2 e3))
-  = admit ()
+  = append_memP_forall (free_vars e1 @ free_vars e2) (free_vars e3);
+    append_memP_forall (free_vars e1) (free_vars e2)
 
 let lem_fv_in_env_pair (g:typ_env) (e1 e2:exp) :
   Lemma ((fv_in_env g e1 /\ fv_in_env g e2) <==> fv_in_env g (EPair e1 e2))
-  = admit ()
+  = append_memP_forall (free_vars e1) (free_vars e2)
 
 let lem_fv_in_env_fst (g:typ_env) (e:exp) :
   Lemma (fv_in_env g (EFst e) <==> fv_in_env g e)
-  = admit ()
+  = ()
 
 let lem_fv_in_env_snd (g:typ_env) (e:exp) :
   Lemma (fv_in_env g (ESnd e) <==>  fv_in_env g e)
-  = admit ()
+  = ()
 
 let lem_fv_in_env_inl (g:typ_env) (e:exp) :
   Lemma (fv_in_env g (EInl e) <==>  fv_in_env g e)
-  = admit ()
+  = ()
 
 let lem_fv_in_env_inr (g:typ_env) (e:exp) :
   Lemma (fv_in_env g (EInr e) <==>  fv_in_env g e)
-  = admit ()
+  = ()
 
+
+#push-options "--split_queries always --z3rlimit 10"
 let lem_fv_in_env_case (g:typ_env) (t1 t2:qType) (e1 e2 e3:exp) :
   Lemma ((fv_in_env g e1 /\ fv_in_env (extend t1 g) e2 /\ fv_in_env (extend t2 g) e3) <==> fv_in_env g (ECase e1 e2 e3))
-  = admit ()
+  =
+  (* Split memP over the appended free variable lists *)
+  append_memP_forall (free_vars_indx e1 0 @ free_vars_indx e2 1) (free_vars_indx e3 1);
+  append_memP_forall (free_vars_indx e1 0) (free_vars_indx e2 1);
+  (* Connect fv_in_env (extend t g) e with free_vars_indx e at depth 1 *)
+  lem_free_vars_indx_shift e2 0;
+  lem_free_vars_indx_shift e3 0
+#pop-options
 
 let lem_fv_in_env_openfile (g:typ_env) (fnm:exp) :
   Lemma (fv_in_env g fnm <==> fv_in_env g (EOpen fnm))
-  = admit ()
+  = ()
 
 let lem_fv_in_env_read (g:typ_env) (fd:exp) :
   Lemma (fv_in_env g fd <==> fv_in_env g (ERead fd))
-  = admit ()
+  = ()
 
 let lem_fv_in_env_write (g:typ_env) (fd msg:exp) :
   Lemma ((fv_in_env g fd /\ fv_in_env g msg) <==> fv_in_env g (EWrite fd msg))
-  = admit ()
+  = append_memP_forall (free_vars fd) (free_vars msg)
 
 let lem_fv_in_env_close (g:typ_env) (fd:exp) :
   Lemma (fv_in_env g fd <==> fv_in_env g (EClose fd))
-  = admit ()
+  = ()
 
 (** STLC Evaluation Environment : variable -> value **)
 let gsub (g:typ_env) (b:bool{b ==> (forall x. None? (g x))}) = (** CA: this b is polluting **)
@@ -352,10 +454,49 @@ let lem_substitution #g #b (s:gsub g b) (t:qType) (v:value) (e:exp)
     (subst (sub_beta v) (subst (sub_elam s) e)) == (subst (gsub_extend s t v) e))
   = admit () (** common lemma **)
 
+(** Helper: substitution is identity on closed expressions.
+    If e has no free variables at binder depth n, and s acts as identity on
+    variables below n, then subst s e == e. *)
+let rec lem_subst_closed_identity #b (s:sub b) (e:exp) (n:nat) :
+  Lemma
+    (requires free_vars_indx e n == [] /\
+              (forall (x:var). x < n ==> s x == EVar x))
+    (ensures subst s e == e)
+    (decreases e) =
+  match e with
+  | EUnit | ETrue | EFalse | EFileDescr _ | EString _ -> ()
+  | EVar _ -> ()
+  | ELam e' ->
+    introduce forall (x:var). x < n+1 ==> sub_elam s x == EVar x with begin
+      introduce _ ==> _ with _. begin
+        if x = 0 then () else ()
+      end
+    end;
+    lem_subst_closed_identity (sub_elam s) e' (n+1)
+  | EFst e' | ESnd e' | EInl e' | EInr e'
+  | ERead e' | EOpen e' | EClose e' ->
+    lem_subst_closed_identity s e' n
+  | EApp e1 e2 | EPair e1 e2 | EWrite e1 e2 ->
+    lem_subst_closed_identity s e1 n;
+    lem_subst_closed_identity s e2 n
+  | EIf e1 e2 e3 ->
+    lem_subst_closed_identity s e1 n;
+    lem_subst_closed_identity s e2 n;
+    lem_subst_closed_identity s e3 n
+  | ECase e1 e2 e3 ->
+    lem_subst_closed_identity s e1 n;
+    introduce forall (x:var). x < n+1 ==> sub_elam s x == EVar x with begin
+      introduce _ ==> _ with _. begin
+        if x = 0 then () else ()
+      end
+    end;
+    lem_subst_closed_identity (sub_elam s) e2 (n+1);
+    lem_subst_closed_identity (sub_elam s) e3 (n+1)
+
 let lem_gsubst_closed_identiy #g #b (s:gsub g b) (e:closed_exp) :
   Lemma (gsubst s e == e)
   [SMTPat (gsubst s e)] =
-  admit ()
+  lem_subst_closed_identity s e 0
 
 module FE = FStar.FunctionalExtensionality
 
